theories/typing/product.v
@@ -10,7 +10,7 @@ Set Default Proof Using "Type".
 Section product.
   Context `{!typeG Σ}.
 
-  Program Definition unit: type unit := {|
+  Program Definition r_unit: type () := {|
     ty_size := 0;  ty_lfts := [];  ty_E := [];
     ty_own _ _ vl := ⌜vl = []⌝%I;  ty_shr _ _ _ _ := True%I
   |}.
@@ -25,15 +25,6 @@ Section product.
     iIntros. iIntros. iApply step_fupdN_intro; [done|]. iIntros "!>!>!>!>!>".
     iExists [], 1%Qp=>/=. iSplit; [iPureIntro; by apply proph_dep_unit|]. by iFrame.
   Qed.
-
-  Global Instance unit_copy: Copy unit.
-  Proof.
-    split; [apply _|]. move=> */=. iIntros "_ _ Na $". iExists 1%Qp, []. iModIntro.
-    iDestruct (na_own_acc with "Na") as "[$ ToNa]"; [solve_ndisj|].
-    rewrite heap_mapsto_vec_nil. do 2 (iSplit; [done|]). iIntros "?_!>". by iApply "ToNa".
-  Qed.
-  Global Instance unit_send: Send unit. Proof. done. Qed.
-  Global Instance unit_sync: Sync unit. Proof. done. Qed.
 
   Lemma split_prod_mt {A B} (vπd: _ A) (vπd': _ B) tid ty ty' q l :
     (l ↦∗{q}: λ vl, ∃wl wl', ⌜vl = wl ++ wl'⌝ ∗
@@ -52,7 +43,7 @@ Section product.
       iFrame "Mt Mt'". iExists wl, wl'. by iFrame.
   Qed.
 
-  Program Definition product2 {A B} (ty: type A) (ty': type B) : type (A * B) :=
+  Program Definition r_prod {A B} (ty: type A) (ty': type B) : type (A * B) :=
     {| ty_size := ty.(ty_size) + ty'.(ty_size);
        ty_lfts := ty.(ty_lfts) ++ ty'.(ty_lfts);  ty_E := ty.(ty_E) ++ ty'.(ty_E);
        ty_own vπd tid vl := (∃ wl wl', ⌜vl = wl ++ wl'⌝ ∗
@@ -120,36 +111,46 @@ Section product.
     iMod ("Close" with "PTok") as "[$$]". by iMod ("Close'" with "PTok'") as "[$$]".
   Qed.
 
-  Global Instance product2_ne {A B} : NonExpansive2 (@product2 A B).
+  Global Instance prod_ne {A B} : NonExpansive2 (@r_prod A B).
   Proof. solve_ne_type. Qed.
 
-  Definition nil_unit: type :1 := mod_ty (λ _, -[]) unit.
+  Definition r_nil_unit: type :1 := <{ const -[] }> r_unit.
 
-  Definition cons_product2 {A B} (ty: type A) (ty': type B)
-    : type (A :* B) := mod_ty pair_to_cons_pair (product2 ty ty').
+  Definition r_cons_prod {A B} (ty: type A) (ty': type B)
+    : type (A :* B) := <{ pair_to_cons_pair }> (r_prod ty ty').
 
-  Global Instance cons_product2_ne {A B} : NonExpansive2 (@cons_product2 A B).
-  Proof. move=> ???????. rewrite /cons_product2. by do 2 f_equiv. Qed.
+  Global Instance cons_prod_ne {A B} : NonExpansive2 (@r_cons_prod A B).
+  Proof. move=> ???????. rewrite /r_cons_prod. by do 2 f_equiv. Qed.
 
-  Fixpoint product {As} (tyl: typel As) : type (xprod As) :=
-    match tyl with +[] => nil_unit | ty +:: tyl' => cons_product2 ty (product tyl') end.
+  Fixpoint r_xprod {As} (tyl: typel As) : type (xprod As) :=
+    match tyl with +[] => r_nil_unit | ty +:: tyl' => r_cons_prod ty (r_xprod tyl') end.
 
-  Global Instance product_ne {As} : NonExpansive (@product As).
+  Global Instance product_ne {As} : NonExpansive (@r_xprod As).
   Proof. move=> ???. elim; [done|]=> */=. by f_equiv. Qed.
 
 End product.
 
-Notation "ty * ty'" := (product2 ty%T ty'%T) : lrust_type_scope.
-Notation ":1" := nil_unit : lrust_type_scope.
-Notation "ty :* ty'" := (cons_product2 ty%T ty'%T) : lrust_type_scope.
-Notation Π := product.
+Notation "()" := (r_unit) : lrust_type_scope.
+Notation "ty * ty'" := (r_prod ty%T ty'%T) : lrust_type_scope.
+Notation ":1" := r_nil_unit : lrust_type_scope.
+Notation "ty :* ty'" := (r_cons_prod ty%T ty'%T) : lrust_type_scope.
+Notation Π := (r_xprod).
 
 Section typing.
   Context `{!typeG Σ}.
 
-  Global Instance product2_lft_morphism {A B C} (T: _ A → _ B) (T' : _ → _ C):
+  Global Instance unit_copy: Copy ().
+  Proof.
+    split; [apply _|]. move=> */=. iIntros "_ _ Na $". iExists 1%Qp, []. iModIntro.
+    iDestruct (na_own_acc with "Na") as "[$ ToNa]"; [solve_ndisj|].
+    rewrite heap_mapsto_vec_nil. do 2 (iSplit; [done|]). iIntros "?_!>". by iApply "ToNa".
+  Qed.
+  Global Instance unit_send: Send (). Proof. done. Qed.
+  Global Instance unit_sync: Sync (). Proof. done. Qed.
+
+  Global Instance prod_lft_morphism {A B C} (T: _ A → _ B) (T': _ → _ C):
     TypeLftMorphism T → TypeLftMorphism T' →
-    TypeLftMorphism (λ ty, product2 (T ty) (T' ty)).
+    TypeLftMorphism (λ ty, T ty * T' ty)%T.
   Proof.
     case=> [α βs E Hα HE|α E Hα HE]; case=> [α' βs' E' Hα' HE'|α' E' Hα' HE'].
     - apply (type_lft_morphism_add _ (α ⊓ α') (βs ++ βs') (E ++ E'))=> ty.
@@ -175,7 +176,7 @@ Section typing.
       + by rewrite /= !elctx_interp_app HE HE'.
   Qed.
 
-  Global Instance product2_type_ne {A B C} (T: _ A → _ B) (T': _ → _ C) :
+  Global Instance prod_type_ne {A B C} (T: _ A → _ B) (T': _ → _ C) :
     TypeNonExpansive T → TypeNonExpansive T' → TypeNonExpansive (λ ty, T ty * T' ty)%T.
   Proof. move=> ??. split=>/=; first apply _.
     - move=> *. f_equiv; by apply type_non_expansive_ty_size.
@@ -184,7 +185,7 @@ Section typing.
       f_equiv; by apply type_non_expansive_ty_shr.
   Qed.
   (* TODO : find a way to avoid this duplication. *)
-  Global Instance product2_type_contractive {A B C} (T: _ A → _ B) (T': _ → _ C) :
+  Global Instance prod_type_contractive {A B C} (T: _ A → _ B) (T': _ → _ C) :
     TypeContractive T → TypeContractive T' → TypeContractive (λ ty, T ty * T' ty)%T.
   Proof. move=> ??. split=>/=; first apply _.
     - move=> *. f_equiv; by apply type_contractive_ty_size.
@@ -193,39 +194,39 @@ Section typing.
       f_equiv; by apply type_contractive_ty_shr.
   Qed.
 
-  Global Instance cons_product2_type_ne {A B C} (T: _ A → _ B) (T': _ → _ C) :
+  Global Instance cons_prod_type_ne {A B C} (T: _ A → _ B) (T': _ → _ C) :
     TypeNonExpansive T → TypeNonExpansive T' → TypeNonExpansive (λ ty, T ty :* T' ty)%T.
   Proof.
-    have ->: (λ ty, T ty :* T' ty)%T =
-      mod_ty pair_to_cons_pair ∘ (λ ty, T ty * T' ty)%T by done.
+    have ->: ((λ ty, T ty :* T' ty) =
+      <{pair_to_cons_pair}> ∘ λ ty, T ty * T' ty)%T by done.
     move=> ??. apply type_ne_ne_compose; apply _.
   Qed.
-  Global Instance cons_product2_type_contractive {A B C} (T: _ A → _ B) (T': _ → _ C) :
+  Global Instance cons_prod_type_contractive {A B C} (T: _ A → _ B) (T': _ → _ C) :
     TypeContractive T → TypeContractive T' → TypeContractive (λ ty, T ty :* T' ty)%T.
   Proof.
-    have ->: (λ ty, T ty :* T' ty)%T =
-      mod_ty pair_to_cons_pair ∘ (λ ty, T ty * T' ty)%T by done.
+    have ->: ((λ ty, T ty :* T' ty) =
+      <{pair_to_cons_pair}> ∘ λ ty, T ty * T' ty)%T by done.
     move=> ??. apply type_contractive_compose_left; apply _.
   Qed.
 
   Global Instance product_type_ne {A Bs} (T: _ A → _ Bs) :
-    TypeListNonExpansive T → TypeNonExpansive (Π ∘ T).
+    TypeListNonExpansive T → TypeNonExpansive (Π ∘ T)%T.
   Proof.
     move=> [Tl [Eq All]].
-    have ->: Π ∘ T = λ ty, Π ((λ _ (T': _ → _), T' ty) +<$>+ Tl).
+    have ->: (Π ∘ T = λ ty, Π ((λ _ (T': _ → _), T' ty) +<$>+ Tl))%T.
     { extensionality ty. by rewrite /= Eq. } clear Eq T.
-    dependent induction All=>/=; by [apply _|apply cons_product2_type_ne].
+    dependent induction All=>/=; by [apply _|apply cons_prod_type_ne].
   Qed.
   Global Instance product_type_ne_cont {A Bs} (T: _ A → _ Bs) :
-    TypeListContractive T → TypeContractive (Π ∘ T).
+    TypeListContractive T → TypeContractive (Π ∘ T)%T.
   Proof.
     move=> [Tl [Eq All]].
-    have ->: Π ∘ T = λ ty, Π ((λ _ (T': _ → _), T' ty) +<$>+ Tl).
+    have ->: (Π ∘ T = λ ty, Π ((λ _ (T': _ → _), T' ty) +<$>+ Tl))%T.
     { extensionality ty. by rewrite /= Eq. } clear Eq T.
-    dependent induction All=>/=; by [apply _|apply cons_product2_type_contractive].
+    dependent induction All=>/=; by [apply _|apply cons_prod_type_contractive].
   Qed.
 
-  Global Instance product2_copy {A B} (ty: _ A) (ty': _ B) :
+  Global Instance prod_copy {A B} (ty: _ A) (ty': _ B) :
     Copy ty → Copy ty' → Copy (ty * ty').
   Proof.
     move=> ??. split; [by apply _|]=>/= > ? HF. iIntros "#LFT [Shr Shr'] Na [Tok Tok']".
@@ -236,8 +237,8 @@ Section typing.
       move: HF. rewrite -plus_assoc shr_locsE_shift. set_solver. }
     iDestruct (na_own_acc with "Na") as "[$ PreNa]".
     { rewrite shr_locsE_shift. set_solver. }
-    case (Qp_lower_bound q q')=> [qq[?[?[->->]]]].
-    iExists qq, (wl ++ wl'). rewrite heap_mapsto_vec_app.
+    case (Qp_lower_bound q q')=> [q''[?[?[->->]]]].
+    iExists q'', (wl ++ wl'). rewrite heap_mapsto_vec_app.
     iDestruct (ty_size_eq with "Own") as ">->".
     iDestruct "Mt" as "[$ Mtr]". iDestruct "Mt'" as "[$ Mtr']".
     iSplitR. { iIntros "!>!>". iExists wl, wl'. iSplit; by [|iSplit]. }
@@ -246,26 +247,26 @@ Section typing.
     iApply ("Close" with "Na [$Mt $Mtr]").
   Qed.
 
-  Global Instance product2_send {A B} (ty: _ A) (ty': _ B) :
+  Global Instance prod_send {A B} (ty: _ A) (ty': _ B) :
     Send ty → Send ty' → Send (ty * ty').
   Proof.
     move=> *?*. iDestruct 1 as (wl wl' ->) "[Own Own']".
     iExists wl, wl'. iSplit; [done|]. iSplitL "Own"; by iApply @send_change_tid.
   Qed.
-  Global Instance product2_sync {A B} (ty: _ A) (ty': _ B) :
+  Global Instance prod_sync {A B} (ty: _ A) (ty': _ B) :
     Sync ty → Sync ty' → Sync (ty * ty').
   Proof.
     move=> *?*. iIntros "[#? #?]". iSplit; by iApply @sync_change_tid.
   Qed.
 
-  Global Instance product_copy {As} (tyl: _ As) : ListCopy tyl → Copy (Π tyl).
+  Global Instance xprod_copy {As} (tyl: _ As) : ListCopy tyl → Copy (Π tyl).
   Proof. elim; apply _. Qed.
-  Global Instance product_send {As} (tyl: _ As) : ListSend tyl → Send (Π tyl).
+  Global Instance xprod_send {As} (tyl: _ As) : ListSend tyl → Send (Π tyl).
   Proof. elim; apply _. Qed.
-  Global Instance product_sync {As} (tyl: _ As) : ListSync tyl → Sync (Π tyl).
+  Global Instance xprod_sync {As} (tyl: _ As) : ListSync tyl → Sync (Π tyl).
   Proof. elim; apply _. Qed.
 
-  Lemma product2_subtype {A B A' B'} E L (f: A → A') (g: B → B') ty1 ty2 ty1' ty2' :
+  Lemma prod_subtype {A B A' B'} E L (f: A → A') (g: B → B') ty1 ty2 ty1' ty2' :
     subtype E L f ty1 ty1' → subtype E L g ty2 ty2' →
     subtype E L (pair_map f g) (ty1 * ty2) (ty1' * ty2').
   Proof.
@@ -281,74 +282,85 @@ Section typing.
     - iIntros "* #[??]". rewrite Eq. iSplit; by [iApply "InShr"|iApply "InShr'"].
   Qed.
 
-  Lemma product2_eqtype {A B A' B'} E L (f: A → A') f' (g: B → B') g' ty1 ty2 ty1' ty2' :
+  Lemma prod_eqtype {A B A' B'} E L (f: A → A') f' (g: B → B') g' ty1 ty2 ty1' ty2' :
     eqtype E L f f' ty1 ty1' → eqtype E L g g' ty2 ty2' →
     eqtype E L (pair_map f g) (pair_map f' g') (ty1 * ty2) (ty1' * ty2').
-  Proof. move=> [??][??]. split; by apply product2_subtype. Qed.
+  Proof. move=> [??][??]. split; by apply prod_subtype. Qed.
 
-  Lemma cons_product2_subtype {A B A' B'} E L (f: A → A') (g: B → B') ty1 ty2 ty1' ty2' :
+  Lemma cons_prod_subtype {A B A' B'} E L (f: A → A') (g: B → B') ty1 ty2 ty1' ty2' :
     subtype E L f ty1 ty1' → subtype E L g ty2 ty2' →
     subtype E L (cons_pair_map f g) (ty1 :* ty2) (ty1' :* ty2').
   Proof.
-    move=> ??. rewrite cons_pair_map_via_pair_map. apply mod_ty_subtype.
-    { apply pair_via_cons_pair. } by apply product2_subtype.
+    move=> ??. rewrite cons_pair_map_via_pair_map.
+    apply mod_ty_subtype; [apply iso|by apply prod_subtype].
   Qed.
 
-  Lemma product_subtype {As Bs} E L (tyl: _ As) (tyl': _ Bs) fl :
+  Lemma xprod_subtype {As Bs} E L (tyl: _ As) (tyl': _ Bs) fl :
     subtypel E L tyl tyl' fl → subtype E L (xprod_map fl) (Π tyl) (Π tyl').
   Proof.
     move=> Subs. dependent induction Subs; [by apply subtype_refl|].
-    by apply cons_product2_subtype.
+    by apply cons_prod_subtype.
   Qed.
 
-  Lemma product_eqtype {As Bs} E L (tyl: _ As) (tyl': _ Bs) fl gl :
+  Lemma xprod_eqtype {As Bs} E L (tyl: _ As) (tyl': _ Bs) fl gl :
     eqtypel E L tyl tyl' fl gl →
     eqtype E L (xprod_map fl) (xprod_map gl) (Π tyl) (Π tyl').
   Proof.
-    move=> /HForallZip_zip [? /HForallZip_flip ?]. by split; apply product_subtype.
+    move=> /HForallZip_zip[? /HForallZip_flip ?]. by split; apply xprod_subtype.
   Qed.
 
-  Lemma outlives_product2 {A B} (ty: _ A) (ty': _ B) ϝ :
+  Lemma outlives_prod {A B} (ty: _ A) (ty': _ B) ϝ :
     ty_outlives_E (ty * ty') ϝ = ty_outlives_E ty ϝ ++ ty_outlives_E ty' ϝ.
   Proof. by rewrite /ty_outlives_E /= fmap_app. Qed.
 
+  Lemma prod_assoc {A B C} E L (ty1: _ A) (ty2: _ B) (ty3: _ C) :
+    eqtype E L pair_assoc pair_assoc' (ty1 * (ty2 * ty3)) ((ty1 * ty2) * ty3).
+  Proof.
+    have Eq: ∀vπ: proph_asn → (A * (B * C)),
+      fst ∘ (fst ∘ (pair_assoc ∘ vπ)) = fst ∘ vπ ∧
+      snd ∘ (fst ∘ (pair_assoc ∘ vπ)) = fst ∘ (snd ∘ vπ) ∧
+      snd ∘ (pair_assoc ∘ vπ) = snd ∘ (snd ∘ vπ).
+    { move=> vπ. split; [|split]; extensionality xyz=>/=; by case (vπ xyz)=> [?[??]]. }
+    apply eqtype_unfold; [apply _|]. iIntros (?) "_!>_/=". iSplit; [iPureIntro; lia|].
+    iSplit; [rewrite (assoc (++)); by iApply lft_equiv_refl|].
+    iSplit; iIntros "!>" (vπ) "*"; move: (Eq vπ)=> [->[->->]].
+    - iSplit.
+      + iDestruct 1 as (wl1 wl23 ->) "[Own1 Own23]".
+        iDestruct "Own23" as (wl2 wl3 ->) "[Own2 Own3]". iExists (wl1 ++ wl2), wl3.
+        iSplit; [by rewrite assoc|]. iFrame "Own3". iExists wl1, wl2. by iFrame.
+      + iDestruct 1 as (wl12 wl3 ->) "[Own12 Own3]".
+        iDestruct "Own12" as (wl1 wl2 ->) "[Own1 Own2]". iExists wl1, (wl2 ++ wl3).
+        iSplit; [by rewrite assoc|]. iFrame "Own1". iExists wl2, wl3. by iFrame.
+    - rewrite -assoc shift_loc_assoc_nat. by iApply (bi.iff_refl True%I).
+  Qed.
+
+  Lemma prod_left_id {A} E L (ty: _ A) :
+    eqtype E L pair_left_id pair_left_id' (() * ty) (ty).
+  Proof.
+    apply eqtype_unfold; [apply _|]. iIntros (?) "_!>_/=". iSplit; [done|].
+    iSplit; [by iApply lft_equiv_refl|].
+    have Eq: ∀vπ: proph_asn → (() * A), pair_left_id ∘ vπ = snd ∘ vπ.
+    { move=> vπ. extensionality π. simpl. by case (vπ π)=> [[]?]. }
+    iSplit; iIntros "!> *"; rewrite Eq; [iSplit|].
+    - by iDestruct 1 as (?? ->->) "Own /=".
+    - iIntros "Own". iExists [], _. by iFrame "Own".
+    - rewrite left_id shift_loc_0. by iApply (bi.iff_refl True%I).
+  Qed.
+
+  Lemma prod_right_id {A} E L (ty: _ A) :
+    eqtype E L pair_right_id pair_right_id' (ty * ()) (ty).
+  Proof.
+    apply eqtype_unfold; [apply _|]. iIntros (?) "_!>_/=".
+    rewrite !right_id. iSplit; [done|]. iSplit; [by iApply lft_equiv_refl|].
+    have Eq: ∀vπ: proph_asn → (A * ()), pair_right_id ∘ vπ = fst ∘ vπ.
+    { move=> vπ. extensionality π. simpl. by case (vπ π)=> [?[]]. }
+    iSplit; iIntros "!> *"; rewrite Eq; [iSplit|].
+    - iDestruct 1 as (?? ->) "[Own ->]". by rewrite right_id.
+    - iIntros "Own". iExists _, []. iFrame "Own". by rewrite right_id.
+    - rewrite right_id. by iApply (bi.iff_refl True%I).
+  Qed.
+
 (*
-  Global Instance prod2_assoc E L : Assoc (eqtype E L) product2.
-  Proof.
-    intros ???. apply eqtype_unfold. iIntros (?) "_ !> _".
-    rewrite /= !(assoc plus) !(assoc app). iSplit; [done|].
-    iSplit; [|iSplit].
-    - iApply lft_equiv_refl.
-    - iIntros "!> *". iSplit; iIntros "H".
-      + iDestruct "H" as (vl1 vl') "(-> & Ho1 & H)".
-        iDestruct "H" as (vl2 vl3) "(-> & Ho2 & Ho3)".
-        iExists _, _. iSplit. by rewrite assoc. iFrame. iExists _, _. by iFrame.
-      + iDestruct "H" as (vl1 vl') "(-> & H & Ho3)".
-        iDestruct "H" as (vl2 vl3) "(-> & Ho1 & Ho2)".
-        iExists _, _. iSplit. by rewrite -assoc. iFrame. iExists _, _. by iFrame.
-    - iIntros "!> *". rewrite assoc shift_loc_assoc_nat. by iApply (bi.iff_refl True%I).
-  Qed.
-
-  Global Instance prod2_unit_leftid E L : LeftId (eqtype E L) unit product2.
-  Proof.
-    intros ty. apply eqtype_unfold. iIntros (?) "_ !> _ /=".
-    setoid_rewrite (left_id True%I bi_sep). setoid_rewrite shift_loc_0.
-    iSplit; [done|iSplit; [|iSplit; iIntros "!> *"; iSplit; iIntros "H //"]].
-    - iApply lft_equiv_refl.
-    - by iDestruct "H" as (? ?) "(-> & -> & ?)".
-    - iExists [], _. eauto.
-  Qed.
-
-  Global Instance prod2_unit_rightid E L : RightId (eqtype E L) unit product2.
-  Proof.
-    intros ty. apply eqtype_unfold. iIntros (?) "_ !> _ /=".
-    setoid_rewrite (right_id True%I bi_sep). rewrite (right_id [] app).
-    iSplit; [done|iSplit; [|iSplit; iIntros "!> *"; iSplit; iIntros "H //"]].
-    - iApply lft_equiv_refl.
-    - iDestruct "H" as (? ?) "(-> & ? & ->)". by rewrite right_id.
-    - iExists _, []. rewrite right_id. eauto.
-  Qed.
-
   Lemma prod_flatten E L tyl1 tyl2 tyl3 :
     eqtype E L (Π(tyl1 ++ Π tyl2 :: tyl3)) (Π(tyl1 ++ tyl2 ++ tyl3)).
   Proof.
